theories/eris/examples/lazy_real.v
@@ -1,0 +1,410 @@
+From clutch.eris Require Export eris error_rules receipt_rules.
+From clutch.eris Require Import presample_many.
+From Coquelicot Require SF_seq Hierarchy.
+From Coquelicot Require Import RInt.
+From clutch.eris Require Import infinite_tape.
+Set Default Proof Using "Type*".
+#[local] Open Scope R.
+
+Section lazy_real.
+
+  (** Program *)
+ Definition get_chunk : val :=
+    λ: "α" "chnk",
+      match: !"chnk" with
+      | NONE =>
+          let: "b" := rand("α") #1 in
+          let: "next" := ref NONEV in
+          let: "val" := ("b", "next") in
+          "chnk" <- SOME "val";;
+          "val"
+      | SOME "val" => "val"
+      end.
+
+  Definition cmpZ : val :=
+    λ: "z1" "z2",
+      if: "z1" < "z2" then #(-1)
+      else
+        if: "z2" < "z1" then #1
+        else #0.
+
+  Definition cmp_list : val :=
+    rec: "cmp_list" "α1" "cl1" "α2" "cl2" :=
+      let: "c1n" := get_chunk "α1" "cl1" in
+      let: "c2n" := get_chunk "α2" "cl2" in
+      let: "res" := cmpZ (Fst "c1n") (Fst "c2n") in
+      if: "res" = #0 then
+        "cmp_list" "α1" (Snd "c1n") "α2" (Snd "c2n")
+      else
+        "res".
+
+  Definition init : val :=
+    λ: <>,
+      let: "hd" := ref NONEV in
+      let: "α" := alloc #1 in
+      ("α", "hd").
+
+  Definition cmp : val :=
+    λ: "lz1" "lz2",
+      (* We short-circuit if the two locations are physically equal to avoid forcing sampling *)
+      if: Snd "lz1" = Snd "lz2" then
+        #0
+      else
+        cmp_list (Fst "lz1") (Snd "lz1") (Fst "lz2") (Snd "lz2").
+
+  Context `{!erisGS Σ}.
+
+  Definition comparison2z c : Z :=
+    match c with
+    | Eq => 0
+    | Lt => -1
+    | Gt => 1
+    end.
+
+  Lemma comparison2z_lt (z1 z2 : Z) :
+    (z1 < z2)%Z →
+    comparison2z (Z.compare z1 z2) = (-1)%Z.
+  Proof.
+    rewrite /comparison2z.
+    case_match eqn:Heq;
+      rewrite ?Z.compare_eq_iff ?Z.compare_gt_iff in Heq; lia.
+  Qed.
+
+  Lemma comparison2z_eq (z1 z2 : Z) :
+    (z1 = z2)%Z →
+    comparison2z (Z.compare z1 z2) = 0%Z.
+  Proof.
+    rewrite /comparison2z.
+    case_match eqn:Heq;
+      rewrite ?Z.compare_lt_iff ?Z.compare_gt_iff in Heq; lia.
+  Qed.
+
+  Lemma comparison2z_gt (z1 z2 : Z) :
+    (z1 > z2)%Z →
+    comparison2z (Z.compare z1 z2) = 1%Z.
+  Proof.
+    rewrite /comparison2z.
+    case_match eqn:Heq;
+      rewrite ?Z.compare_eq_iff ?Z.compare_lt_iff in Heq; lia.
+  Qed.
+
+  Lemma wp_cmpZ (z1 z2 : Z) E :
+    ⟨⟨⟨ True ⟩⟩⟩
+      cmpZ #z1 #z2 @ E
+    ⟨⟨⟨ RET #(comparison2z (Z.compare z1 z2)); True%I ⟩⟩⟩.
+  Proof.
+    iIntros (Φ) "_ HΦ". rewrite /cmpZ.
+    destruct (Z.compare_spec z1 z2).
+    - wp_pures; case_bool_decide; [lia|].
+      wp_pures; case_bool_decide; [lia|].
+      wp_pures. iApply "HΦ"; eauto.
+    - wp_pures; case_bool_decide; [|lia].
+      wp_pures. iApply "HΦ"; eauto.
+    - wp_pures; case_bool_decide; [lia|].
+      wp_pures; case_bool_decide; [|lia].
+      wp_pures. iApply "HΦ"; eauto.
+  Qed.
+
+  Fixpoint chunk_list (l : loc) (zs : list (fin 2)) : iProp Σ :=
+    match zs with
+    | [] => l ↦ NONEV
+    | z :: zs =>
+        ∃ l' : loc, l ↦ SOMEV (#z, #l') ∗ chunk_list l' zs
+  end.
+
+  Definition chunk_and_tape_seq α l (f: nat → (fin 2)) : iProp Σ :=
+    ∃ zs f', ⌜f = append_bin_seq zs f' ⌝∗ chunk_list l zs ∗ infinite_tape α f'.
+
+  Definition lazy_real (v : val) (r : R) : iProp Σ :=
+    ∃ (l : loc) (α : loc) (f : nat → (fin 2)),
+      ⌜v = (#lbl:α, #l)%V⌝ ∗
+      ⌜ r = seq_bin_to_R f ⌝ ∗
+      chunk_and_tape_seq α l f.
+
+  Lemma chunk_list_hd_acc l zs :
+    chunk_list l zs -∗
+    (∃ v, l ↦ v ∗ (l ↦ v -∗ chunk_list l zs)).
+  Proof.
+    destruct zs.
+    - simpl. iIntros. iExists _. iFrame. eauto.
+    - simpl. iIntros "(%&H1&H2)". iExists _. iFrame.
+      iIntros "H". iExists _. iFrame.
+  Qed.
+
+  Lemma chunk_and_tape_list_ne (l1 l2 α1 α2 : loc) f1 f2 :
+    chunk_and_tape_seq α1 l1 f1 -∗ chunk_and_tape_seq α2 l2 f2 -∗ ⌜l1 ≠ l2⌝.
+  Proof.
+    iIntros "(% & % & _ & Hl1 & _) (% & % & _ & Hl2 & _)".
+    iDestruct (chunk_list_hd_acc with "Hl1") as (?) "[Hl1 _]".
+    iDestruct (chunk_list_hd_acc with "Hl2") as (?) "[Hl2 _]".
+    iApply (ghost_map_elem_ne with "Hl1 Hl2").
+  Qed.
+
+  Lemma chunk_and_tape_list_cons_chunk (l l' : loc) (z : fin _) (f : nat → (fin 2)) α :
+    l ↦ SOMEV (#z, #l') -∗
+    chunk_and_tape_seq α l' f -∗
+    chunk_and_tape_seq α l (cons_bin_seq z f).
+  Proof.
+    iIntros "Hl Htape". iDestruct "Htape" as (zs1 zs2 Heq) "(Hchunks&Hlist)".
+    iExists (z :: zs1), zs2.
+    iSplit.
+    { rewrite Heq /=//. }
+    iSplitL "Hl Hchunks".
+    { rewrite /=. iExists l'. iFrame. }
+    iFrame.
+  Qed.
+
+  (*
+  Lemma rwp_get_chunk α l E :
+    ⟨⟨⟨ chunk_and_tape_seq α l f ⟩⟩⟩
+      get_chunk #lbl:α #l @ E
+    ⟨⟨⟨ (z : fin 2) (l' : loc), RET (#z, #l');
+        chunk_and_tape_list α l' [] ∗
+        (∀ zs, chunk_and_tape_list α l' zs -∗ chunk_and_tape_list α l (z :: zs)) ⟩⟩⟩.
+  Proof.
+    iIntros (Ψ) "(%zs1 & %zs2 & %Heq & Hl & Hα) HΨ".
+    rewrite /get_chunk.
+    symmetry in Heq. apply app_nil in Heq as [-> ->].
+    wp_pures.
+    wp_load. wp_pures.
+    wp_apply (rwp_rand_tape_empty with "Hα").
+    iIntros (n) "Hα". wp_pures. wp_alloc l' as "Hl'". wp_pures. wp_store.
+    iModIntro. iApply "HΨ".
+    iSplitR "Hl".
+    { iExists [], []. iSplit; [done|]. iFrame. }
+    { iIntros (?) "Htail". iApply (chunk_and_tape_list_cons_chunk with "Hl Htail"). }
+  Qed.
+   *)
+
+  Lemma wp_get_chunk_cons z f α l E :
+    ⟨⟨⟨ chunk_and_tape_seq α l (cons_bin_seq z f) ⟩⟩⟩
+      get_chunk #lbl:α #l @ E
+    ⟨⟨⟨ l', RET (#z, #l');
+        chunk_and_tape_seq α l' f ∗
+       (∀ f, chunk_and_tape_seq α l' f -∗ chunk_and_tape_seq α l (cons_bin_seq z f)) ⟩⟩⟩.
+  Proof.
+    iIntros (Ψ) "(%zs1 & %zs2 & %Heq & Hl & Hα) HΨ".
+    rewrite /get_chunk.
+    wp_pures.
+    destruct zs1 as [| z' zs1'].
+    - wp_load. wp_pures.
+      rewrite /= in Heq.
+      assert (zs2 = cons_bin_seq z f) as ->.
+      { rewrite Heq. eauto. }
+      wp_apply (wp_rand_infinite_tape_cons with "Hα").
+      iIntros "Hα".
+      wp_pures. wp_alloc l' as "Hl'". wp_pures. wp_store.
+      iModIntro. iApply "HΨ". iSplitR "Hl".
+      { iExists [], f. iSplit; [done|]. iFrame. }
+      { iIntros (?) "Htail". iApply (chunk_and_tape_list_cons_chunk with "[$] [$]"). }
+    - rewrite /=. iDestruct "Hl" as "(%l' & Hl & Hl')".
+      wp_load. wp_pures.
+      assert (z = z').
+      { cut (cons_bin_seq z f O = append_bin_seq (z' :: zs1') zs2 O); first done.
+        rewrite Heq //=. }
+      subst.
+      iModIntro. iApply "HΨ".
+      iSplitR "Hl".
+      { iExists _, _. iFrame. apply cons_bin_seq_inv in Heq as (Heq1&Heq2). auto. }
+      { iIntros (?) "Htail". iApply (chunk_and_tape_list_cons_chunk with "[$] [$]"). }
+  Qed.
+
+  Lemma wp_cmp_list α1 α2 l1 l2 E zs1 zs2 :
+    ⟨⟨⟨ chunk_and_tape_seq α1 l1 zs1 ∗
+        chunk_and_tape_seq α2 l2 zs2 ⟩⟩⟩
+      cmp_list #lbl:α1 #l1 #lbl:α2 #l2 @ E
+    ⟨⟨⟨ (z : Z), RET #z;
+        (⌜ z = (-1)%Z ∧ (seq_bin_to_R zs1 <= seq_bin_to_R zs2)%R ⌝ ∨
+         ⌜ z = 1%Z  ∧ (seq_bin_to_R zs2 <= seq_bin_to_R zs2)%R ⌝) ∗
+        chunk_and_tape_seq α1 l1 zs1 ∗
+        chunk_and_tape_seq α2 l2 zs2
+         ⟩⟩⟩.
+  Proof.
+  Abort.
+  (*
+    iIntros (?).
+    iInduction zs1 as [|z1 zs1] "IH" forall (l1 l2 zs2 b).
+    - iInduction zs2 as [|z2 zs2] "IH" forall (l1 l2 b).
+      + iIntros (Ψ) "(Hspec & Hl1 & Hl2) HΨ".
+        destruct N; [lia|].
+        wp_apply (rwp_cmp_list_nil_nil with "[$Hspec $Hl1 $Hl2]").
+        iIntros (b' z1 z2 zs) "(Hspec & % & Hl1 & Hl2)".
+        iApply ("HΨ").
+        iFrame. iSplit.
+        { iPureIntro. apply prefix_nil. }
+        iSplit.
+        { iPureIntro. apply prefix_nil. }
+        iSplit; [done|].
+        iPureIntro. lia.
+      + iIntros (Ψ) " (Hspec & Hl1 & Hl2) HΨ".
+        rewrite {2}/cmp_list. wp_pures.
+        wp_apply (rwp_get_chunk_nil with "Hl1").
+        iIntros (z1 l1') "(Hl1' & Hl1)". wp_pures.
+        wp_apply (rwp_get_chunk_cons with "Hl2").
+        iIntros (l2') "[Hl2' Hl2]".
+        wp_pures.
+        wp_apply wp_cmpZ; [done|]; iIntros "_".
+        wp_pures.
+        destruct (Z.compare_spec z1 z2)
+          as [? | Hl | Hgt]; simplify_eq=>/=.
+        * do 3 wp_pure _.
+          wp_apply ("IH" with "[$Hspec $Hl1' $Hl2']").
+          iIntros (???????)  "(Hl1' & Hl2' & % & % & Hspec)".
+          iSpecialize ("Hl1" with "Hl1'").
+          iSpecialize ("Hl2" with "Hl2'").
+          rewrite 2!app_comm_cons.
+          iApply "HΨ". iFrame.
+          iSplit; [iPureIntro; apply prefix_nil|].
+          iPureIntro. by apply prefix_cons.
+        * wp_pures.
+          iSpecialize ("Hl1" with "Hl1'").
+          iSpecialize ("Hl2" with "Hl2'").
+          iModIntro.
+          iSpecialize ("HΨ" $! _ _ z1 z2 [] [] zs2).
+          rewrite comparison2z_lt //.
+          iApply "HΨ".
+          iFrame.
+          iSplit; [iPureIntro; apply prefix_nil|].
+          iSplit; [done|].
+          iSplit; [|iPureIntro; lia].
+          iPureIntro. intros ->; lia.
+        * wp_pures.
+          iSpecialize ("Hl1" with "Hl1'").
+          iSpecialize ("Hl2" with "Hl2'").
+          iModIntro.
+          iSpecialize ("HΨ" $! _ _ z1 z2 [] [] zs2).
+          rewrite comparison2z_gt; [|lia].
+          iApply "HΨ".
+          iFrame. iPureIntro.
+          split; [apply prefix_nil|].
+          split; [done|].
+          split; [|lia]. intros ->; lia.
+    - destruct zs2 as [|z2 zs2].
+      + iIntros (Ψ) "(Hspec & Hl1 & Hl2) HΨ".
+        rewrite {2}/cmp_list. wp_pures.
+        wp_apply (rwp_get_chunk_cons with "Hl1").
+        iIntros (l1') "(Hl1' & Hl1)". wp_pures.
+        wp_apply (rwp_get_chunk_nil with "Hl2").
+        iIntros (z2 l2') "[Hl2' Hl2]".
+        wp_pures.
+        wp_apply wp_cmpZ; [done|]; iIntros "_".
+        wp_pures.
+        destruct (Z.compare_spec z1 z2)
+          as [? | Hlt | Hgt]; simplify_eq=>/=.
+        * do 3 wp_pure _.
+          wp_apply ("IH" with "[$Hspec $Hl1' $Hl2']").
+          iIntros (???????)  "(Hl1' & Hl2' & % & % & Hspec)".
+          iSpecialize ("Hl1" with "Hl1'").
+          iSpecialize ("Hl2" with "Hl2'").
+          rewrite 2!app_comm_cons.
+          iApply "HΨ". iFrame.
+          iPureIntro.
+          split; [by apply prefix_cons|].
+          apply prefix_nil.
+        * wp_pures.
+          iSpecialize ("Hl1" with "Hl1'").
+          iSpecialize ("Hl2" with "Hl2'").
+          iModIntro.
+          iSpecialize ("HΨ" $! _ _ z1 z2 [] zs1 []).
+          rewrite comparison2z_lt //.
+          iApply "HΨ".
+          iFrame. iPureIntro.
+          split; [done|].
+          split; [apply prefix_nil|].
+          split; [|lia]. intros ->; lia.
+        * wp_pures.
+          iSpecialize ("Hl1" with "Hl1'").
+          iSpecialize ("Hl2" with "Hl2'").
+          iModIntro.
+          iSpecialize ("HΨ" $! _ _ z1 z2 [] zs1 []).
+          rewrite comparison2z_gt; [|lia].
+          iApply "HΨ".
+          iFrame. iPureIntro.
+          split; [done|].
+          split; [apply prefix_nil|].
+          split; [|lia]. intros ->; lia.
+      + iIntros (Ψ) "(Hspec & Hl1 & Hl2) HΨ".
+        rewrite {2}/cmp_list. wp_pures.
+        wp_apply (rwp_get_chunk_cons with "Hl1").
+        iIntros (l1') "(Hl1' & Hl1)". wp_pures.
+        wp_apply (rwp_get_chunk_cons with "Hl2").
+        iIntros (l2') "[Hl2' Hl2]".
+        wp_pures.
+        wp_apply wp_cmpZ; [done|]; iIntros "_".
+        wp_pures.
+        destruct (Z.compare_spec z1 z2)
+          as [? | Hlt | Hgt]; simplify_eq=>/=.
+        * do 3 wp_pure _.
+          wp_apply ("IH" with "[$Hspec $Hl1' $Hl2']").
+          iIntros (???????)  "(Hl1' & Hl2' & % & % & Hspec)".
+          iSpecialize ("Hl1" with "Hl1'").
+          iSpecialize ("Hl2" with "Hl2'").
+          rewrite 2!app_comm_cons.
+          iApply "HΨ". iFrame.
+          iPureIntro.
+          split; by apply prefix_cons.
+        * wp_pures.
+          iSpecialize ("Hl1" with "Hl1'").
+          iSpecialize ("Hl2" with "Hl2'").
+          iModIntro.
+          iSpecialize ("HΨ" $! _ _ z1 z2 [] zs1 zs2).
+          rewrite comparison2z_lt //.
+          iApply "HΨ".
+          iFrame. iPureIntro.
+          split; [done|]. split; [done|]. split; [|lia]. intros ->; lia.
+        * wp_pures.
+          iSpecialize ("Hl1" with "Hl1'").
+          iSpecialize ("Hl2" with "Hl2'").
+          iModIntro.
+          iSpecialize ("HΨ" $! _ _ z1 z2 [] zs1 zs2).
+          rewrite comparison2z_gt; [|lia].
+          iApply "HΨ".
+          iFrame. iPureIntro.
+          split; [done|]. split; [done|]. split; [|lia]. intros ->; lia.
+  Qed.
+
+  Lemma rwp_init E :
+    ⟨⟨⟨ True ⟩⟩⟩
+      init #() @ E
+    ⟨⟨⟨ v, RET v; lazy_no [] v ⟩⟩⟩.
+  Proof.
+    iIntros (Ψ) "_ HΨ".
+    wp_rec.
+    wp_alloc l as "Hl".
+    wp_pures.
+    wp_apply rwp_alloc_tape; [done|].
+    iIntros (α) "Hα".
+    wp_pures.
+    iModIntro.
+    iApply "HΨ".
+    iExists _, _. iSplit; [done|].
+    iExists [], []. by iFrame.
+  Qed.
+
+  Definition cmps (N : nat) : iProp Σ := ∃ b M, specF (b, b, M) ∗ ⌜M ≥ N⌝.
+
+  Lemma rwp_cmp E v1 v2 zs1 zs2 N :
+    (N > 0)%nat →
+    ⟨⟨⟨ lazy_no zs1 v1 ∗ lazy_no zs2 v2 ∗ cmps N ⟩⟩⟩
+      cmp v1 v2 @ E
+    ⟨⟨⟨ (z : Z) zs1' zs2', RET #z;
+        lazy_no (zs1 ++ zs1') v1 ∗ lazy_no (zs2 ++ zs2') v2 ∗ cmps (N - 1) ⟩⟩⟩.
+  Proof.
+    iIntros (? Ψ) "((%l1 & %α1 & -> & Hl1) & (%l2 & %α2 & -> & Hl2) & (% & % & Hcmps & %)) HΨ".
+    wp_rec. wp_pures.
+    iDestruct (chunk_and_tape_list_ne with "Hl1 Hl2") as %?.
+    rewrite bool_decide_eq_false_2; [|by intros [=]].
+    wp_pures.
+    destruct M; [lia|].
+    wp_apply (rwp_cmp_list with "[$Hcmps $Hl1 $Hl2]"); [lia|].
+    iIntros (???????) "(Hl1 & Hl2 & [%zs1'' ->] & [%zs2'' ->] & % & Hs & %)".
+    iApply "HΨ".
+    iSplitL "Hl1".
+    { iExists _, _. by iFrame. }
+    iSplitL "Hl2".
+    { iExists _, _. by iFrame. }
+    iFrame. eauto with lia.
+  Qed.
+   *)
+
+End lazy_real.
